OpenvmFv/Equivalence/LoadStore.lean
@@ -866,6 +866,372 @@ namespace Equivalence.LoadStore
     . exact h_memory.2.1.2.2.2.2.1
     . exact h_memory.2.1.2.2.2.2.2
 
+  lemma lw_spec_of_get_instruction_fields_part_15 [Field ExtF]
+    (air : Valid_VmAirWrapper_loadstore FBB ExtF)
+    (row : ℕ)
+    (h_row : row ≤ air.last_row)
+    (h_is_valid : air.core.is_valid row 0 = 1)
+    (h_opcode : air.core.expected_opcode row 0 = 528)
+    (h_constraints : VmAirWrapper_loadstore.constraints.allHold air row h_row)
+    (h_bus_assumptions : VmAirWrapper_loadstore.constraints.assumptionsPerRow air row)
+    (h_bus_wellformedness : VmAirWrapper_loadstore.constraints.wf_propertiesToAssumePerRow air row)
+  :
+    BitVec.ofNat 32 (air.adapter.from_state.pc row 0).val + 4#32 =
+    BitVec.ofNat 32 (air.to_pc row 0).val
+  := by
+    simp [
+      Valid_VmAirWrapper_loadstore.to_pc
+    ]
+    have h_execution := h_bus_assumptions.1
+    simp [
+      VmAirWrapper_loadstore_constraint_and_interaction_simplification,
+      h_is_valid
+    ] at h_execution
+    rewrite [Fin.val_add, Nat.mod_eq_of_lt, BitVec.ofNat_add]
+    . simp
+    . omega
+
+  lemma lw_spec_of_get_instruction_fields_part_16 [Field ExtF]
+    (air : Valid_VmAirWrapper_loadstore FBB ExtF)
+    (row : ℕ)
+    (h_row : row ≤ air.last_row)
+    (h_is_valid : air.core.is_valid row 0 = 1)
+    (h_opcode : air.core.expected_opcode row 0 = 528)
+    (h_constraints : VmAirWrapper_loadstore.constraints.allHold air row h_row)
+    (h_bus_assumptions : VmAirWrapper_loadstore.constraints.assumptionsPerRow air row)
+    (h_bus_wellformedness : VmAirWrapper_loadstore.constraints.wf_propertiesToAssumePerRow air row)
+    (h1 : (air.adapter.imm row 0).val % 256 < 2 ^ 8)
+    (h2 : (air.adapter.imm row 0).val / 256 % 256 < 2 ^ 8)
+    (h3 : (air.adapter.imm_extended_limb row 0).val % 256 < 2 ^ 8)
+    (h4 : (air.adapter.imm_extended_limb row 0).val / 256 % 256 < 2 ^ 8)
+    (h5 : (air.adapter.rs1_data_0 row 0).val % 256 < 2 ^ 8)
+    (h6 : (air.adapter.rs1_data_1 row 0).val % 256 < 2 ^ 8)
+    (h7 : (air.adapter.rs1_data_2 row 0).val % 256 < 2 ^ 8)
+    (h8 : (air.adapter.rs1_data_3 row 0).val % 256 < 2 ^ 8)
+  :
+    ↑(air.read_ptr row 0) =
+    (
+      U32.toNat #v[
+        { toFin := ⟨↑(air.adapter.imm row 0) % 256, h1⟩ },
+        { toFin := ⟨↑(air.adapter.imm row 0) / 256 % 256, h2⟩ },
+        { toFin := ⟨↑(air.adapter.imm_extended_limb row 0) % 256, h3⟩ },
+        { toFin := ⟨↑(air.adapter.imm_extended_limb row 0) / 256 % 256, h4⟩ }
+      ] +
+      U32.toNat #v[
+        { toFin := ⟨↑(air.adapter.rs1_data_0 row 0) % 256, h5⟩ },
+        { toFin := ⟨↑(air.adapter.rs1_data_1 row 0) % 256, h6⟩ },
+        { toFin := ⟨↑(air.adapter.rs1_data_2 row 0) % 256, h7⟩ },
+        { toFin := ⟨↑(air.adapter.rs1_data_3 row 0) % 256, h8⟩ }
+      ]
+    ) % 4294967296
+  := by
+    simp only [U32.toNat]
+    rewrite [
+      BitVec.toNat_ofFin,
+      BitVec.toNat_ofFin,
+      BitVec.toNat_ofFin,
+      BitVec.toNat_ofFin,
+      BitVec.toNat_ofFin,
+      BitVec.toNat_ofFin,
+      BitVec.toNat_ofFin,
+      BitVec.toNat_ofFin
+    ]
+    simp
+    have := Load.read_ptr_of_opcode_528 air row h_opcode h_row h_constraints h_is_valid
+    rewrite [this]; clear this
+    have h_mem_ptr := Load.mem_ptr_eq_imm_plus_rs1 air row h_opcode h_row h_constraints h_is_valid h_bus_wellformedness
+    have h_imm_sign_extend := Load.imm_sign_extend_of_opcode_528 air row h_opcode h_is_valid h_bus_wellformedness
+    rewrite [h_imm_sign_extend] at h_mem_ptr
+    rewrite [BitVec.toNat_eq] at h_mem_ptr
+    simp [-BitVec.toNat_add] at h_mem_ptr
+    rewrite [BitVec.toNat_add] at h_mem_ptr
+    simp at h_mem_ptr
+    rewrite [Nat.mod_eq_of_lt (by omega)] at h_mem_ptr
+    rewrite [h_mem_ptr]; clear h_mem_ptr
+    congr
+    rewrite [BitVec.toNat_ofFin]
+    simp
+    have (x y: ℕ) :
+      (BitVec.setWidth 32 (BitVec.ofNat 16 x)) <<< 16 +
+      (BitVec.setWidth 32 (BitVec.ofNat 16 y)) =
+      (BitVec.ofNat 16 x) ++ (BitVec.ofNat 16 y)
+    := by bv_decide
+    rewrite [←this]; clear this
+    rewrite [BitVec.toNat_add]
+    simp
+    have (x: ℕ) :
+      x % 65536 =
+      256 * (x / 256) % 65536 + x % 256
+    := by
+      rewrite (occs := .pos [1]) [
+        ←Nat.div_add_mod x 256
+      ]
+      rw [
+        Nat.add_mod,
+        Nat.mod_eq_of_lt (by omega),
+        @Nat.mod_eq_of_lt (x % 256) _ (by omega)
+      ]
+    rewrite [@Nat.mod_eq_of_lt (_ % 65536)]
+    simp [Nat.shiftLeft_eq]
+    rewrite [@Nat.mod_eq_of_lt _ 4294967296 (by omega)]
+    rewrite [this]
+    . omega
+    . omega
+
+  lemma lw_spec_of_get_instruction_fields_part_17 [Field ExtF]
+    (air : Valid_VmAirWrapper_loadstore FBB ExtF)
+    (row : ℕ)
+    (h_row : row ≤ air.last_row)
+    (h_is_valid : air.core.is_valid row 0 = 1)
+    (h_opcode : air.core.expected_opcode row 0 = 528)
+    (h_constraints : VmAirWrapper_loadstore.constraints.allHold air row h_row)
+    (h_bus_assumptions : VmAirWrapper_loadstore.constraints.assumptionsPerRow air row)
+    (h_bus_wellformedness : VmAirWrapper_loadstore.constraints.wf_propertiesToAssumePerRow air row)
+    (h1 : (air.adapter.imm row 0).val % 256 < 2 ^ 8)
+    (h2 : (air.adapter.imm row 0).val / 256 % 256 < 2 ^ 8)
+    (h3 : (air.adapter.imm_extended_limb row 0).val % 256 < 2 ^ 8)
+    (h4 : (air.adapter.imm_extended_limb row 0).val / 256 % 256 < 2 ^ 8)
+  :
+    BitVec.signExtend 32
+    (BitVec.setWidth 12
+      (U32.toBV
+        #v[
+          { toFin := ⟨↑(air.adapter.imm row 0) % 256, h1⟩ },
+          { toFin := ⟨↑(air.adapter.imm row 0) / 256 % 256, h2⟩ },
+          { toFin := ⟨↑(air.adapter.imm_extended_limb row 0) % 256, h3⟩ },
+          { toFin := ⟨↑(air.adapter.imm_extended_limb row 0) / 256 % 256, h4⟩ }
+        ]
+      )
+    ) =
+    U32.toBV
+      #v[
+        { toFin := ⟨↑(air.adapter.imm row 0) % 256, h1⟩ },
+        { toFin := ⟨↑(air.adapter.imm row 0) / 256 % 256, h2⟩ },
+        { toFin := ⟨↑(air.adapter.imm_extended_limb row 0) % 256, h3⟩ },
+        { toFin := ⟨↑(air.adapter.imm_extended_limb row 0) / 256 % 256, h4⟩ }
+      ]
+  := by
+    have := Load.imm_sign_extend_of_opcode_528 air row h_opcode h_is_valid h_bus_wellformedness
+    simp [U32.toBV]
+    have (bv1 bv2 bv3 bv4: BitVec 8) :
+      BitVec.setWidth 12 (bv1 ++ bv2 ++ bv3 ++ bv4) =
+      BitVec.setWidth 12 (bv3 ++ bv4)
+    := by bv_decide
+    rewrite [this]; clear this
+    -- combine the two halves of imm into BitVec.ofNat 16 imm
+    have h_imm_range := Load.imm_range_of_opcode_528 air row h_opcode h_is_valid h_bus_wellformedness
+    have h_split_imm := split_bitvec_16_to_8s h_imm_range
+    simp [BitVec.ofNat, Nat.cast] at h_split_imm
+    unfold NatCast.natCast Fin.NatCast.instNatCast Fin.ofNat at h_split_imm
+    dsimp at h_split_imm
+    simp (disch := omega) [Nat.mod_eq_of_lt] at h_split_imm
+    simp (disch := omega) [Nat.mod_eq_of_lt]
+    have (a b c d: BitVec 8) : a ++ b ++ c ++ d = (a ++ b) ++ (c ++ d) := by grind
+    rewrite [this]
+    simp [←h_split_imm]
+    have :
+      BitVec.signExtend 32 (BitVec.setWidth 12 (BitVec.ofNat 16 (air.adapter.imm row 0))) =
+      BitVec.signExtend 32 (BitVec.ofNat 16 (air.adapter.imm row 0))
+    := by
+      have h_transpile := h_bus_wellformedness.2.2.2
+      simp [
+        VmAirWrapper_loadstore_constraint_and_interaction_simplification,
+        h_is_valid,
+        Interaction.ReadInstructionBusEntry.operand_properties
+      ] at h_transpile
+      obtain ⟨
+        instruction,
+        multiplciity,
+        data,
+        ⟨h_instruction, _, _, h_data_opcode, _, _, h_data_imm, _⟩
+      ⟩ := h_transpile
+      rewrite [←h_data_imm]
+      have := Transpiler.transpiler_opcode_528 h_instruction
+      simp [h_data_opcode, h_opcode] at this
+      have h_alignment := Transpiler.pc_aligned_of_some h_instruction
+      obtain
+        ⟨_, imm, rs1, rd, h_instruction_load, _⟩ |
+        ⟨_, imm, rs1, h_instruction_load⟩
+      := this
+      all_goals {
+        rewrite [h_instruction_load] at h_instruction
+        unfold Transpiler.transpile_op at h_instruction
+        rewrite [ite_cond_eq_true _ _ (eq_true h_alignment)] at h_instruction
+        dsimp at h_instruction
+        simp [-Vector.mk_eq] at h_instruction
+        simp (disch := omega) [←h_instruction.2, Transpiler.utof, Transpiler.sign_extend_16, Nat.mod_eq_of_lt]
+        bv_decide
+      }
+    convert this using 1
+    . simp [BitVec.ofNat, Nat.cast]
+      unfold NatCast.natCast Fin.NatCast.instNatCast Fin.ofNat
+      dsimp
+      simp (disch := omega) [Nat.mod_eq_of_lt]
+    . have h_imm_extended_range := Load.imm_extend_range_of_opcode_528 air row h_row h_constraints h_is_valid
+      have h_split_imm_extended := split_bitvec_16_to_8s h_imm_extended_range
+      simp [BitVec.ofNat, Nat.cast] at h_split_imm_extended
+      unfold NatCast.natCast Fin.NatCast.instNatCast Fin.ofNat at h_split_imm_extended
+      dsimp at h_split_imm_extended
+      simp (disch := omega) [Nat.mod_eq_of_lt] at h_split_imm_extended
+      simp (disch := omega) [Nat.mod_eq_of_lt]
+      rewrite [←h_split_imm_extended]
+      have := Load.imm_sign_extend_of_opcode_528 air row h_opcode h_is_valid h_bus_wellformedness
+      rewrite [this]
+      simp [BitVec.ofNat, Nat.cast]
+      unfold NatCast.natCast Fin.NatCast.instNatCast Fin.ofNat
+      dsimp
+      simp (disch := omega) [Nat.mod_eq_of_lt]
+
+  lemma lw_spec_of_get_instruction_fields_part_18 [Field ExtF]
+    (air : Valid_VmAirWrapper_loadstore FBB ExtF)
+    (row : ℕ)
+    (h_row : row ≤ air.last_row)
+    (h_is_valid : air.core.is_valid row 0 = 1)
+    (h_opcode : air.core.expected_opcode row 0 = 528)
+    (h_constraints : VmAirWrapper_loadstore.constraints.allHold air row h_row)
+    (h_bus_assumptions : VmAirWrapper_loadstore.constraints.assumptionsPerRow air row)
+    (h_bus_wellformedness : VmAirWrapper_loadstore.constraints.wf_propertiesToAssumePerRow air row)
+    (h1 : (air.adapter.imm row 0).val % 256 < 2 ^ 8)
+    (h2 : (air.adapter.imm row 0).val / 256 % 256 < 2 ^ 8)
+    (h3 : (air.adapter.imm_extended_limb row 0).val % 256 < 2 ^ 8)
+    (h4 : (air.adapter.imm_extended_limb row 0).val / 256 % 256 < 2 ^ 8)
+  :
+    U32.toBV
+    #v[
+      { toFin := ⟨↑(air.adapter.imm row 0) % 256, h1⟩ },
+      { toFin := ⟨↑(air.adapter.imm row 0) / 256 % 256, h2⟩ },
+      { toFin := ⟨↑(air.adapter.imm_extended_limb row 0) % 256, h3⟩ },
+      { toFin := ⟨↑(air.adapter.imm_extended_limb row 0) / 256 % 256, h4⟩ }
+    ] =
+    BitVec.signExtend 32 (BitVec.ofNat 16 ↑(air.adapter.imm row 0))
+  := by
+    simp [U32.toBV]
+    have := Load.imm_sign_extend_of_opcode_528 air row h_opcode h_is_valid h_bus_wellformedness
+    rewrite [this]
+    have (a b c d: BitVec 8) : a ++ b ++ c ++ d = (a ++ b) ++ (c ++ d) := by grind
+    rewrite [this]; clear this
+    congr
+    . have := Nat.div_add_mod (air.adapter.imm_extended_limb row 0).val 256
+      have :
+        BitVec.ofNat 16 (air.adapter.imm_extended_limb row 0).val =
+        BitVec.ofNat 16 (
+          256 * ((air.adapter.imm_extended_limb row 0).val / 256) +
+          (air.adapter.imm_extended_limb row 0).val % 256
+        )
+      := by
+        rw (occs := .pos [1]) [←this]
+      rewrite [this]; clear this; clear this; clear this
+      rewrite [BitVec.ofNat_add, BitVec.ofNat_mul]
+      have : (air.adapter.imm_extended_limb row 0).val / 256 < 256 := by
+        have := Load.imm_extend_range_of_opcode_528 air row h_row h_constraints h_is_valid
+        omega
+      simp [Nat.mod_eq_of_lt this]
+      have (bv1 bv2: BitVec 8) :
+        256#16 * BitVec.setWidth 16 bv1 + BitVec.setWidth 16 bv2 =
+        bv1 ++ bv2
+      := by bv_decide
+      rewrite [←this]
+      congr
+      . simp [
+          ← BitVec.toNat_inj,
+          - BitVec.toNat_ofFin
+        ]
+        rw [BitVec.toNat_ofFin]
+      . simp [
+          ← BitVec.toNat_inj,
+          - BitVec.toNat_ofFin
+        ]
+        rw [BitVec.toNat_ofFin]
+    . have := Nat.div_add_mod (air.adapter.imm row 0).val 256
+      have :
+        BitVec.ofNat 16 (air.adapter.imm row 0).val =
+        BitVec.ofNat 16 (
+          256 * ((air.adapter.imm row 0).val / 256) +
+          (air.adapter.imm row 0).val % 256
+        )
+      := by
+        rw (occs := .pos [1]) [←this]
+      rewrite [this]; clear this; clear this; clear this
+      rewrite [BitVec.ofNat_add, BitVec.ofNat_mul]
+      have : (air.adapter.imm row 0).val / 256 < 256 := by
+        have := Load.imm_range_of_opcode_528 air row h_opcode h_is_valid h_bus_wellformedness
+        omega
+      simp [Nat.mod_eq_of_lt this]
+      have (bv1 bv2: BitVec 8) :
+        256#16 * BitVec.setWidth 16 bv1 + BitVec.setWidth 16 bv2 =
+        bv1 ++ bv2
+      := by bv_decide
+      rewrite [←this]
+      congr <;> {
+        unfold BitVec.setWidth BitVec.setWidth' BitVec.toNat
+        simp [BitVec.ofNat]
+        refine BitVec.eq_of_toNat_eq ?_
+        simp
+        omega
+      }
+
+  lemma lw_spec_of_get_instruction_fields_part_19 [Field ExtF]
+    (air : Valid_VmAirWrapper_loadstore FBB ExtF)
+    (row : ℕ)
+    (h_row : row ≤ air.last_row)
+    (h_is_valid : air.core.is_valid row 0 = 1)
+    (h_opcode : air.core.expected_opcode row 0 = 528)
+    (h_constraints : VmAirWrapper_loadstore.constraints.allHold air row h_row)
+    (h_bus_assumptions : VmAirWrapper_loadstore.constraints.assumptionsPerRow air row)
+    (h_bus_wellformedness : VmAirWrapper_loadstore.constraints.wf_propertiesToAssumePerRow air row)
+    (h1 : (air.adapter.imm row 0).val % 256 < 2 ^ 8)
+    (h2 : (air.adapter.imm row 0).val / 256 % 256 < 2 ^ 8)
+    (h3 : (air.adapter.imm_extended_limb row 0).val % 256 < 2 ^ 8)
+    (h4 : (air.adapter.imm_extended_limb row 0).val / 256 % 256 < 2 ^ 8)
+  :
+    air.adapter.imm_sign row 0 =
+    ↑(
+      U32.toBV
+        #v[
+          { toFin := ⟨↑(air.adapter.imm row 0) % 256, h1⟩ },
+          { toFin := ⟨↑(air.adapter.imm row 0) / 256 % 256, h2⟩ },
+          { toFin := ⟨↑(air.adapter.imm_extended_limb row 0) % 256, h3⟩ },
+          { toFin := ⟨↑(air.adapter.imm_extended_limb row 0) / 256 % 256, h4⟩ }
+        ]
+    ).msb.toNat
+  := by
+    have := Load.imm_sign_of_opcode_528 air row h_bus_wellformedness h_is_valid h_opcode
+    rewrite [this]; clear this
+    simp [U32.toBV]
+    have (bv1 bv2 bv3 bv4: BitVec 8) : (bv1 ++ bv2 ++ bv3 ++ bv4).msb = bv1.msb := by bv_decide
+    simp [this]
+    have := Load.imm_extend_range_of_opcode_528 air row h_row h_constraints h_is_valid
+    have :
+      (air.adapter.imm_extended_limb row 0).val / 256 % 256 =
+      (air.adapter.imm_extended_limb row 0).val / 256
+    := by
+      omega
+    simp [this]
+    have h_sign_extend := Load.imm_sign_extend_of_opcode_528 air row h_opcode h_is_valid h_bus_wellformedness
+    have (bv1 bv2: BitVec 32): bv1 = bv2 → bv1.msb = bv2.msb := by intro h; grind
+    apply this at h_sign_extend
+    have (bv: BitVec 16) : (bv.signExtend 32).msb = bv.msb := by bv_decide
+    rewrite [this] at h_sign_extend
+    rewrite [h_sign_extend]
+    have (bv1 bv2: BitVec 16): (bv1 ++ bv2).msb = bv1.msb := by bv_decide
+    rewrite [this]
+    have (a b : Bool) : (a.toNat: FBB) = (b.toNat: FBB) ↔ a = b := by cases a <;> cases b <;> decide
+    rewrite [this]
+    simp [BitVec.msb, BitVec.getMsbD, Nat.testBit]
+    rewrite [Nat.mod_eq_of_lt (by omega)]
+    unfold getElem BitVec.instGetElemNatBoolLt
+    simp only [BitVec.getLsb, Nat.testBit]
+    simp
+    rewrite [
+      Nat.mod_eq_of_lt (by omega),
+      Nat.mod_eq_of_lt (by omega),
+      Nat.shiftRight_eq_div_pow,
+      Nat.shiftRight_eq_div_pow,
+    ]
+    simp
+    rewrite [Nat.div_div_eq_div_mul]
+    simp
+
   set_option maxHeartbeats 0 in
   lemma lw_spec_of_get_instruction_fields [Field ExtF]
     (air : Valid_VmAirWrapper_loadstore FBB ExtF)
@@ -888,7 +1254,7 @@ namespace Equivalence.LoadStore
       get_instruction_fields_row,
       -BitVec.toNat_add
     ]
-    rw [BitVec.toNat_add]
+    rewrite [BitVec.toNat_add]
     simp
 
     rewrite [allHold_allRows] at h_constraints
@@ -912,242 +1278,14 @@ namespace Equivalence.LoadStore
     . exact lw_spec_of_get_instruction_fields_part_12 air row h_row h_is_valid h_opcode h_constraints h_bus_assumptions h_bus_wellformedness
     . exact lw_spec_of_get_instruction_fields_part_13 air row h_row h_is_valid h_opcode h_constraints h_bus_assumptions h_bus_wellformedness
     . exact lw_spec_of_get_instruction_fields_part_14 air row h_row h_is_valid h_opcode h_constraints h_bus_assumptions h_bus_wellformedness
-    . simp [
-        Valid_VmAirWrapper_loadstore.to_pc
-      ]
-      have h_execution := h_bus_assumptions.1
-      simp [
-        VmAirWrapper_loadstore_constraint_and_interaction_simplification,
-        h_is_valid
-      ] at h_execution
-      rewrite [Fin.val_add, Nat.mod_eq_of_lt, BitVec.ofNat_add]
-      . simp
-      . omega
+    . exact lw_spec_of_get_instruction_fields_part_15 air row h_row h_is_valid h_opcode h_constraints h_bus_assumptions h_bus_wellformedness
     . exact Load.read_as_of_opcode_528 air row h_opcode h_row h_constraints h_is_valid
     . exact Load.write_as_of_opcode_528 air row h_opcode h_row h_constraints h_is_valid
-    . have := Load.read_ptr_of_opcode_528 air row h_opcode h_row h_constraints h_is_valid
-      rewrite [this]; clear this
-      have h_mem_ptr := Load.mem_ptr_eq_imm_plus_rs1 air row h_opcode h_row h_constraints h_is_valid h_bus_wellformedness
-      have h_imm_sign_extend := Load.imm_sign_extend_of_opcode_528 air row h_opcode h_is_valid h_bus_wellformedness
-      rewrite [h_imm_sign_extend] at h_mem_ptr
-      rewrite [BitVec.toNat_eq] at h_mem_ptr
-      simp [-BitVec.toNat_add] at h_mem_ptr
-      rw [BitVec.toNat_add] at h_mem_ptr
-      simp at h_mem_ptr
-      rewrite [Nat.mod_eq_of_lt (by omega)] at h_mem_ptr
-      rewrite [h_mem_ptr]; clear h_mem_ptr
-      congr
-      simp only [
-        U32.toNat,
-        Vector.getElem_mk,
-        List.getElem_toArray,
-        List.getElem_cons_zero,
-        List.getElem_cons_succ
-      ]
-      repeat rw [BitVec.toNat_ofFin]
-      simp
-      have (x y: ℕ) :
-        (BitVec.setWidth 32 (BitVec.ofNat 16 x)) <<< 16 +
-        (BitVec.setWidth 32 (BitVec.ofNat 16 y)) =
-        (BitVec.ofNat 16 x) ++ (BitVec.ofNat 16 y)
-      := by bv_decide
-      rewrite [←this]; clear this
-      rw [BitVec.toNat_add]
-      simp
-      have (x: ℕ) :
-        x % 65536 =
-        256 * (x / 256) % 65536 + x % 256
-      := by
-        rewrite (occs := .pos [1]) [
-          ←Nat.div_add_mod x 256
-        ]
-        rw [
-          Nat.add_mod,
-          Nat.mod_eq_of_lt (by omega),
-          @Nat.mod_eq_of_lt (x % 256) _ (by omega)
-        ]
-      rewrite [@Nat.mod_eq_of_lt (_ % 65536)]
-      simp [Nat.shiftLeft_eq]
-      rewrite [@Nat.mod_eq_of_lt _ 4294967296 (by omega)]
-      rewrite [this]
-      . omega
-      . omega
+    . apply lw_spec_of_get_instruction_fields_part_16 air row h_row h_is_valid h_opcode h_constraints h_bus_assumptions h_bus_wellformedness
     . exact Load.write_ptr_of_opcode_528 air row h_opcode h_row h_constraints h_is_valid
-    . have := Load.imm_sign_extend_of_opcode_528 air row h_opcode h_is_valid h_bus_wellformedness
-      simp [U32.toBV]
-      have (bv1 bv2 bv3 bv4: BitVec 8) :
-        BitVec.setWidth 12 (bv1 ++ bv2 ++ bv3 ++ bv4) =
-        BitVec.setWidth 12 (bv3 ++ bv4)
-      := by bv_decide
-      rewrite [this]; clear this
-      -- combine the two halves of imm into BitVec.ofNat 16 imm
-      have h_imm_range := Load.imm_range_of_opcode_528 air row h_opcode h_is_valid h_bus_wellformedness
-      have h_split_imm := split_bitvec_16_to_8s h_imm_range
-      simp [BitVec.ofNat, Nat.cast] at h_split_imm
-      unfold NatCast.natCast Fin.NatCast.instNatCast Fin.ofNat at h_split_imm
-      dsimp at h_split_imm
-      simp (disch := omega) [Nat.mod_eq_of_lt] at h_split_imm
-      simp (disch := omega) [Nat.mod_eq_of_lt]
-      have (a b c d: BitVec 8) : a ++ b ++ c ++ d = (a ++ b) ++ (c ++ d) := by grind
-      rewrite [this]
-      simp [←h_split_imm]
-      have :
-        BitVec.signExtend 32 (BitVec.setWidth 12 (BitVec.ofNat 16 (air.adapter.imm row 0))) =
-        BitVec.signExtend 32 (BitVec.ofNat 16 (air.adapter.imm row 0))
-      := by
-        have h_transpile := h_bus_wellformedness.2.2.2
-        simp [
-          VmAirWrapper_loadstore_constraint_and_interaction_simplification,
-          h_is_valid,
-          Interaction.ReadInstructionBusEntry.operand_properties
-        ] at h_transpile
-        obtain ⟨
-          instruction,
-          multiplciity,
-          data,
-          ⟨h_instruction, _, _, h_data_opcode, _, _, h_data_imm, _⟩
-        ⟩ := h_transpile
-        rewrite [←h_data_imm]
-        have := Transpiler.transpiler_opcode_528 h_instruction
-        simp [h_data_opcode, h_opcode] at this
-        have h_alignment := Transpiler.pc_aligned_of_some h_instruction
-        obtain
-          ⟨_, imm, rs1, rd, h_instruction_load, _⟩ |
-          ⟨_, imm, rs1, h_instruction_load⟩
-        := this
-        all_goals {
-          rewrite [h_instruction_load] at h_instruction
-          unfold Transpiler.transpile_op at h_instruction
-          rewrite [ite_cond_eq_true _ _ (eq_true h_alignment)] at h_instruction
-          dsimp at h_instruction
-          simp [-Vector.mk_eq] at h_instruction
-          simp (disch := omega) [←h_instruction.2, Transpiler.utof, Transpiler.sign_extend_16, Nat.mod_eq_of_lt]
-          bv_decide
-        }
-      convert this using 1
-      . simp [BitVec.ofNat, Nat.cast]
-        unfold NatCast.natCast Fin.NatCast.instNatCast Fin.ofNat
-        dsimp
-        simp (disch := omega) [Nat.mod_eq_of_lt]
-      . have h_imm_extended_range := Load.imm_extend_range_of_opcode_528 air row h_row h_constraints h_is_valid
-        have h_split_imm_extended := split_bitvec_16_to_8s h_imm_extended_range
-        simp [BitVec.ofNat, Nat.cast] at h_split_imm_extended
-        unfold NatCast.natCast Fin.NatCast.instNatCast Fin.ofNat at h_split_imm_extended
-        dsimp at h_split_imm_extended
-        simp (disch := omega) [Nat.mod_eq_of_lt] at h_split_imm_extended
-        simp (disch := omega) [Nat.mod_eq_of_lt]
-        rewrite [←h_split_imm_extended]
-        have := Load.imm_sign_extend_of_opcode_528 air row h_opcode h_is_valid h_bus_wellformedness
-        rewrite [this]
-        simp [BitVec.ofNat, Nat.cast]
-        unfold NatCast.natCast Fin.NatCast.instNatCast Fin.ofNat
-        dsimp
-        simp (disch := omega) [Nat.mod_eq_of_lt]
-    . simp [U32.toBV]
-      have := Load.imm_sign_extend_of_opcode_528 air row h_opcode h_is_valid h_bus_wellformedness
-      rewrite [this]
-      have (a b c d: BitVec 8) : a ++ b ++ c ++ d = (a ++ b) ++ (c ++ d) := by grind
-      rewrite [this]; clear this
-      congr
-      . have := Nat.div_add_mod (air.adapter.imm_extended_limb row 0).val 256
-        have :
-          BitVec.ofNat 16 (air.adapter.imm_extended_limb row 0).val =
-          BitVec.ofNat 16 (
-            256 * ((air.adapter.imm_extended_limb row 0).val / 256) +
-            (air.adapter.imm_extended_limb row 0).val % 256
-          )
-        := by
-          rw (occs := .pos [1]) [←this]
-        rewrite [this]; clear this; clear this; clear this
-        rewrite [BitVec.ofNat_add, BitVec.ofNat_mul]
-        have : (air.adapter.imm_extended_limb row 0).val / 256 < 256 := by
-          have := Load.imm_extend_range_of_opcode_528 air row h_row h_constraints h_is_valid
-          omega
-        simp [Nat.mod_eq_of_lt this]
-        have (bv1 bv2: BitVec 8) :
-          256#16 * BitVec.setWidth 16 bv1 + BitVec.setWidth 16 bv2 =
-          bv1 ++ bv2
-        := by bv_decide
-        rewrite [←this]
-        congr
-        . simp [
-            ← BitVec.toNat_inj,
-            - BitVec.toNat_ofFin
-          ]
-          rw [BitVec.toNat_ofFin]
-        . simp [
-            ← BitVec.toNat_inj,
-            - BitVec.toNat_ofFin
-          ]
-          rw [BitVec.toNat_ofFin]
-      . have := Nat.div_add_mod (air.adapter.imm row 0).val 256
-        have :
-          BitVec.ofNat 16 (air.adapter.imm row 0).val =
-          BitVec.ofNat 16 (
-            256 * ((air.adapter.imm row 0).val / 256) +
-            (air.adapter.imm row 0).val % 256
-          )
-        := by
-          rw (occs := .pos [1]) [←this]
-        rewrite [this]; clear this; clear this; clear this
-        rewrite [BitVec.ofNat_add, BitVec.ofNat_mul]
-        have : (air.adapter.imm row 0).val / 256 < 256 := by
-          have := Load.imm_range_of_opcode_528 air row h_opcode h_is_valid h_bus_wellformedness
-          omega
-        simp [Nat.mod_eq_of_lt this]
-        have (bv1 bv2: BitVec 8) :
-          256#16 * BitVec.setWidth 16 bv1 + BitVec.setWidth 16 bv2 =
-          bv1 ++ bv2
-        := by bv_decide
-        rewrite [←this]
-        congr <;> {
-          unfold BitVec.setWidth BitVec.setWidth' BitVec.toNat
-          simp [BitVec.ofNat]
-          refine BitVec.eq_of_toNat_eq ?_
-          simp
-          omega
-          done
-        }
-      done
-
-
-    all_goals
-      sorry
-
-#exit
-
-    . have := Load.imm_sign_of_opcode_528 air row h_bus_wellformedness h_is_valid h_opcode
-      rewrite [this]; clear this
-      simp [U32.toBV]
-      have (bv1 bv2 bv3 bv4: BitVec 8) : (bv1 ++ bv2 ++ bv3 ++ bv4).msb = bv1.msb := by bv_decide
-      simp [this]
-      have := Load.imm_extend_range_of_opcode_528 air row h_row h_constraints h_is_valid
-      have :
-        (air.adapter.imm_extended_limb row 0).val / 256 % 256 =
-        (air.adapter.imm_extended_limb row 0).val / 256
-      := by
-        omega
-      simp [this]
-      have h_sign_extend := Load.imm_sign_extend_of_opcode_528 air row h_opcode h_is_valid h_bus_wellformedness
-      have (bv1 bv2: BitVec 32): bv1 = bv2 → bv1.msb = bv2.msb := by intro h; grind
-      apply this at h_sign_extend
-      have (bv: BitVec 16) : (bv.signExtend 32).msb = bv.msb := by bv_decide
-      rewrite [this] at h_sign_extend
-      rewrite [h_sign_extend]
-      have (bv1 bv2: BitVec 16): (bv1 ++ bv2).msb = bv1.msb := by bv_decide
-      rewrite [this]
-      simp [BitVec.ofNat, BitVec.msb, BitVec.getMsbD, Nat.testBit]
-      rewrite [
-        Nat.mod_eq_of_lt (by omega),
-        Nat.mod_eq_of_lt (by omega),
-        Nat.mod_eq_of_lt (by omega),
-        Nat.shiftRight_eq_div_pow,
-        Nat.shiftRight_eq_div_pow,
-      ]
-      simp
-      rewrite [Nat.div_div_eq_div_mul]
-      simp
-      done
+    . apply lw_spec_of_get_instruction_fields_part_17 air row h_row h_is_valid h_opcode h_constraints h_bus_assumptions h_bus_wellformedness
+    . apply lw_spec_of_get_instruction_fields_part_18 air row h_row h_is_valid h_opcode h_constraints h_bus_assumptions h_bus_wellformedness
+    . apply lw_spec_of_get_instruction_fields_part_19 air row h_row h_is_valid h_opcode h_constraints h_bus_assumptions h_bus_wellformedness
     . have h_transpile := h_bus_wellformedness.2.2.2
       simp [
         VmAirWrapper_loadstore_constraint_and_interaction_simplification,
